Moved some stuff into Quantum_Extra2

Quantum_Extra.thy
@@ -132,21 +132,6 @@ lemma compatible_selfbutter_join:
   apply (subst register_pair_apply[symmetric, where F=R and G=S])
   using assms by auto
 
-definition empty_var :: \<open>'a::{CARD_1,enum} update \<Rightarrow> 'b::finite update\<close> where
-  "empty_var a = one_dim_iso a *\<^sub>C id_cblinfun"
-
-lemma register_empty_var[simp]: \<open>register empty_var\<close>
-  unfolding register_def empty_var_def
-  by (auto simp add: clinearI scaleC_left.add)
-
-lemma empty_var_compatible[simp]: \<open>register X \<Longrightarrow> compatible empty_var X\<close>
-  apply (rule compatibleI)
-  using [[simproc del: Laws_Quantum.compatibility_warn]]
-  by (auto simp: empty_var_def)
-
-lemma empty_var_compatible'[simp]: \<open>register X \<Longrightarrow> compatible X empty_var\<close>
-  using compatible_sym empty_var_compatible by blast
-
 lemma register_mult':
   assumes \<open>register F\<close>
   shows \<open>F a *\<^sub>V F b *\<^sub>V c = F (a o\<^sub>C\<^sub>L b) *\<^sub>V c\<close>
